rocq/theories/TypeSystem/AlphaRoots.v
@@ -270,6 +270,19 @@ Inductive typed_env_roots_shadow_safe
         (params_of_tys param_tys) Σ' R' arg_roots ->
       typed_env_roots_shadow_safe env Ω n R Σ (ECallExpr callee args) ret
         Σ' R' (root_set_union roots_callee (root_sets_union arg_roots))
+  | TERS_CallExpr_TypeForall : forall R R1 R' Σ Σ1 Σ' callee args u
+        type_params bounds body_ty param_tys ret_inner type_args arg_roots roots_callee,
+      (forall fname caps, callee <> EMakeClosure fname caps) ->
+      typed_env_roots_shadow_safe env Ω n R Σ callee
+        (MkTy u (TTypeForall type_params bounds body_ty)) Σ1 R1 roots_callee ->
+      ty_core body_ty = TFn param_tys ret_inner ->
+      check_type_forall_bounds env bounds type_args = None ->
+      typed_args_roots_shadow_safe env Ω n R1 Σ1 args
+        (params_of_tys (map (subst_type_params_ty type_args) param_tys))
+        Σ' R' arg_roots ->
+      typed_env_roots_shadow_safe env Ω n R Σ (ECallExpr callee args)
+        (subst_type_params_ty type_args ret_inner)
+        Σ' R' (root_set_union roots_callee (root_sets_union arg_roots))
   | TERS_Struct : forall R R' Σ Σ' sname lts args fields sdef roots,
       Program.lookup_struct sname env = Some sdef ->
       Datatypes.length lts = Program.struct_lifetimes sdef ->
@@ -944,6 +957,32 @@ Proof.
     exists R20, (root_set_union roots_callee0 (root_sets_union arg_roots0)).
     split; [| split; [| split]].
     + eapply TERS_CallExpr_Closure; eauto.
+    + exact HnsR20.
+    + exact HR20.
+    + eapply root_set_equiv_trans.
+      * apply root_set_union_equiv.
+        -- exact Hroots_callee0.
+        -- eapply root_set_equiv_trans.
+           ++ apply root_sets_union_equiv. exact Harg_roots0.
+           ++ apply root_set_equiv_sym. apply root_sets_instantiate_union_equiv.
+      * apply root_set_equiv_sym. apply root_set_instantiate_union_equiv.
+  - intros R R1 R' Σ Σ1 Σ' callee args u type_params bounds body_ty
+      param_tys ret_inner type_args arg_roots roots_callee
+      Hnot_mc Hcallee IHcallee Hbody Htf_bounds Hargs IHargs Hfresh R0 HnsR HnsR0 HR0.
+    rewrite expr_local_store_names_call_expr in Hfresh.
+    apply root_subst_images_exclude_names_app_inv in Hfresh.
+    destruct Hfresh as [Hfresh_callee Hfresh_args].
+    destruct (IHcallee Hfresh_callee R0 HnsR HnsR0 HR0)
+      as [R10 [roots_callee0 [Hcallee0 [HnsR10 [HR10 Hroots_callee0]]]]].
+    assert (Hns_R1 : root_env_no_shadow R1).
+    { eapply typed_env_roots_no_shadow.
+      - eapply typed_env_roots_shadow_safe_roots. exact Hcallee.
+      - exact HnsR. }
+    destruct (IHargs Hfresh_args R10 Hns_R1 HnsR10 HR10)
+      as [R20 [arg_roots0 [Hargs0 [HnsR20 [HR20 Harg_roots0]]]]].
+    exists R20, (root_set_union roots_callee0 (root_sets_union arg_roots0)).
+    split; [| split; [| split]].
+    + eapply TERS_CallExpr_TypeForall; eauto.
     + exact HnsR20.
     + exact HR20.
     + eapply root_set_equiv_trans.
