rocq/theories/TypeSystem/TypeSafetyCallFrameShadowSafe.v
@@ -230,6 +230,12 @@ Proof.
     + exact n0.
     + apply H. eapply root_env_tail_fresh_names_app_l. exact H1.
     + apply H0. eapply root_env_tail_fresh_names_app_r. exact H1.
+  - eapply TERS_CallExpr_TypeForall.
+    + exact n0.
+    + apply H. eapply root_env_tail_fresh_names_app_l. exact H1.
+    + exact e.
+    + exact e0.
+    + apply H0. eapply root_env_tail_fresh_names_app_r. exact H1.
   - eapply TERS_Struct; eauto.
   - eapply TERS_Enum; eauto.
   - pose proof (root_env_tail_fresh_names_app_l _ _ _ H2) as Hfresh_scrut.
